src/tree/BinTreeIntClara.dfy
@@ -1,0 +1,857 @@
+include "../../src/Order.dfy"
+
+
+datatype tree<A> = Empty | Node(left: tree<A>, data: A, right: tree<A>)
+
+function method Leaf<A>(d: A): tree<A>
+{
+  Node(Empty, d, Empty)
+}
+
+function method elems<A>(t: tree<A>): set<A>
+  ensures t.Empty? ==> elems(t) == {}
+  ensures !t.Empty? ==> elems(t) == elems(t.left) + {t.data} + elems(t.right)
+{
+  match t {
+    case Empty => {}
+    case Node(l, x, r) => elems(l) + {x} + elems(r)
+  }
+}
+
+function method melems<A>(t: tree<A>): multiset<A>
+{
+  match t {
+    case Empty => multiset{}
+    case Node(l, x, r) => melems(l) + multiset{x} + melems(r)
+  }
+}
+
+function method fmap<A, B>(t: tree<A>, f: A -> B): tree<B>
+{
+  match t {
+    case Empty() => Empty()
+    case Node(l, x, r) => Node(fmap(l, f), f(x), fmap(r, f))
+  }
+}
+
+function method preorder<A>(t: tree<A>): seq<A>
+{
+  match t {
+    case Empty => []
+    case Node(l, x, r) => [x] + preorder(l) + preorder(r)
+  }
+}
+
+function method inorder<A>(t: tree<A>): seq<A>
+{
+  match t {
+    case Empty => []
+    case Node(l, x, r) => inorder(l) + [x] + inorder(r)
+  }
+}
+
+function method revinorder<A>(t: tree<A>): seq<A>
+{
+  match t {
+    case Empty => []
+    case Node(l, x, r) => revinorder(r) + [x] + revinorder(l)
+  }
+}
+
+function method postorder<A>(t: tree<A>): seq<A>
+{
+  match t {
+    case Empty => []
+    case Node(l, x, r) => postorder(l) + postorder(r) + [x]
+  }
+}
+
+function method size<A>(t: tree<A>): nat
+{
+  |preorder(t)|
+}
+
+function method max(x: int, y: int): int
+{
+  if x < y then
+    y
+  else
+    x
+}
+
+function method depth<A>(t: tree<A>): nat
+{
+  match t {
+    case Empty => 0
+    case Node(l, x, r) => max(depth(l), depth(r)) + 1
+  }
+}
+
+datatype Color = Red | Black
+
+type K = int
+type V = int
+
+class TNode {
+  var key: K;
+  var value: V;
+  var left: TNode?;
+  var right: TNode?;
+
+  var color: Color;
+
+  constructor(l: TNode?, k: K, v: V, r: TNode?)
+    ensures left == l
+    ensures key == k
+    ensures value == v
+    ensures right == r
+  {
+    key := k;
+    value := v;
+    left := l;
+    right := r;
+  }
+
+  constructor Leaf(k: K, v: V)
+  {
+    key := k;
+    value := v;
+    left := null;
+    right := null;
+  }
+}
+
+class Tree {
+  var root: TNode?;
+  ghost var skeleton: tree<TNode>;
+
+  function Repr(): set<object>
+    reads this
+  {
+    elems(skeleton)
+  }
+
+  static predicate ValidRec(node: TNode?, sk: tree<TNode>)
+    // reads elems(sk)
+    reads set x | x in elems(sk) :: x`left
+    reads set x | x in elems(sk) :: x`right
+  {
+    match sk {
+      case Empty => node == null
+      case Node(l, x, r) =>
+        && x == node
+        && x !in elems(l)
+        && x !in elems(r)
+        && elems(l) !! elems(r)
+        && ValidRec(node.left, l)
+        && ValidRec(node.right, r)
+    }
+  }
+
+  predicate Valid()
+    reads this, Repr()
+  {
+    ValidRec(root, skeleton)
+  }
+
+ 
+  /*static function ModelRec(sk: tree<TNode>): tree<K>
+    reads set x | x in elems(sk) :: x`key
+  {
+    match sk {
+      case Empty() => Empty()
+      case Node(l, n, r) => Node(ModelRec(l), n.key, ModelRec(r))
+    }
+  }
+
+  function Model(): tree<K>  // TODO: tree<(K, V)>
+    reads this, elems(skeleton)
+    requires Valid()
+  {
+    ModelRec(skeleton)
+  }*/
+
+  static function MapModelRec(sk: tree<TNode>): map<K, V>
+    reads set x | x in elems(sk) :: x`key
+    reads set x | x in elems(sk) :: x`value
+    ensures forall n | n in elems(sk) :: n.key in MapModelRec(sk)
+    ensures sk==Empty() ==> MapModelRec(sk)==map[]
+    ensures sk!=Empty ==>MapModelRec(sk) == (MapModelRec(sk.left)+MapModelRec(sk.right))[sk.data.key:=sk.data.value]
+  {
+    match sk {
+      case Empty() => map[]
+      case Node(l, n, r) => (MapModelRec(l) + MapModelRec(r))[n.key := n.value]
+    }
+  }
+
+
+  function MapModel(): map<K, V>
+    reads this, elems(skeleton)
+    requires Valid()
+  {
+    MapModelRec(skeleton)
+  }
+
+  constructor()
+    ensures Valid()
+    ensures fresh(Repr())
+    //ensures Model() == Empty
+    ensures MapModel()==map[]
+  {
+    root := null;
+    skeleton := Empty;
+  }
+
+  predicate SearchTree()
+    reads this, Repr()
+    requires Valid()
+  {
+    SearchTreeRec(skeleton)
+  }
+
+  static predicate SearchTreeRec(sk: tree<TNode>)
+    reads set x | x in elems(sk) :: x`key
+  {
+    match sk {
+      case Empty() => true
+      case Node(l, n, r) =>
+        && (forall m | m in elems(l) :: m.key < n.key)
+        && (forall m | m in elems(r) :: n.key < m.key)
+        && SearchTreeRec(l)
+        && SearchTreeRec(r)
+    }
+  }
+
+
+  lemma ModelRelationWithSkeleton(k: K, v: V)
+    requires Valid()
+    requires SearchTree()
+    ensures k in MapModel() && MapModel()[k] == v <==> exists n | n in elems(skeleton) :: n.key == k && n.value == v
+  {
+    if k in MapModel() && MapModel()[k] == v {
+      ModelRelationWithSkeletonRecR(root, skeleton, k, v);
+    }
+    if exists n | n in elems(skeleton) :: n.key == k && n.value == v {
+      ModelRelationWithSkeletonRecL(root, skeleton, k, v);
+    }
+  }
+
+  static lemma ModelRelationWithSkeletonRecR(node: TNode?, sk: tree<TNode>, k: K, v: V)
+    requires ValidRec(node, sk)
+    requires SearchTreeRec(sk)
+    requires k in MapModelRec(sk)
+    requires MapModelRec(sk)[k] == v
+    ensures (exists n | n in elems(sk) :: n.key == k && n.value == v)
+  {}
+
+  static lemma ModelRelationWithSkeletonRecL(node: TNode?, sk: tree<TNode>, k: K, v: V)
+    requires ValidRec(node, sk)
+    requires SearchTreeRec(sk)
+    requires (exists n | n in elems(sk) :: n.key == k && n.value == v)
+    ensures k in MapModelRec(sk)
+    ensures MapModelRec(sk)[k] == v
+  {
+    match sk {
+      case Empty => {}
+      case Node(l, n, r) => {
+        if n.key == k {
+        } else if k < n.key {
+          assert k in MapModelRec(l);
+
+          assert forall m | m in elems(r) :: n.key != m.key;
+          if k in MapModelRec(r) {
+            ModelRelationWithSkeletonKeyRecR(n.right, r, k);
+            assert false;
+          }
+          assert k !in MapModelRec(r);
+
+          assert MapModelRec(sk)[k] == v;
+        } else if n.key < k {
+        } else {
+          assert false;
+        }
+      }
+    }
+  }
+
+  lemma ModelRelationWithSkeletonKey(k: K)
+    requires Valid()
+    requires SearchTree()
+    ensures k in MapModel() <==> exists n | n in elems(skeleton) :: n.key == k
+  {
+    if k in MapModel() {
+      ModelRelationWithSkeletonKeyRecR(root, skeleton, k);
+    }
+    if exists n | n in elems(skeleton) :: n.key == k {
+      ModelRelationWithSkeletonKeyRecL(root, skeleton, k);
+    }
+  }
+
+ static lemma ModelRelationWithSkeletonKeyRec(node: TNode?, sk: tree<TNode>,k: K)
+    requires ValidRec(node, sk)
+    requires SearchTreeRec(sk)
+    ensures k in MapModelRec(sk) <==> (exists n | n in elems(sk) :: n.key == k)
+  {
+    if k in MapModelRec(sk) {
+      ModelRelationWithSkeletonKeyRecR(node, sk, k);
+    }
+    if exists n | n in elems(sk) :: n.key == k {
+      ModelRelationWithSkeletonKeyRecL(node, sk, k);
+    }
+  }
+
+  static lemma ModelRelationWithSkeletonKeyRecR(node: TNode?, sk: tree<TNode>, k: K)
+    requires ValidRec(node, sk)
+    requires SearchTreeRec(sk)
+    requires k in MapModelRec(sk)
+    ensures (exists n | n in elems(sk) :: n.key == k)
+  {}
+
+  static lemma ContraModelRelationWithSkeletonKeyRecR(node: TNode?, sk: tree<TNode>, k: K)
+    requires ValidRec(node, sk)
+    requires SearchTreeRec(sk)
+    requires forall m | m in elems(sk) :: k != m.key;
+    ensures k !in MapModelRec(sk)
+  {
+      if k in MapModelRec(sk) {
+        ModelRelationWithSkeletonKeyRecR(node, sk, k);
+        assert false;
+      }
+      assert k !in MapModelRec(sk);
+  }
+
+  static lemma ModelRelationWithSkeletonKeyRecL(node: TNode?, sk: tree<TNode>, k: K)
+    requires ValidRec(node, sk)
+    requires SearchTreeRec(sk)
+    requires (exists n | n in elems(sk) :: n.key == k)
+    ensures k in MapModelRec(sk)
+  {
+    match sk {
+      case Empty => {}
+      case Node(l, n, r) => {}
+    }
+  }
+
+
+  function method isEmpty(): bool
+    reads this, Repr()
+    requires Valid()
+    ensures isEmpty() <==> MapModel() == map[]
+  { root==null }  
+
+  function method Size():nat
+    reads this, Repr()
+    requires Valid()
+    ensures Size() == |MapModel()|
+  //TO  DO:añadir tamaño
+
+  static method {:verify false} SearchRec(n: TNode, ghost sk: tree<TNode>, k: K) returns (b:bool, ghost z:TNode)
+    requires ValidRec(n, sk)
+    requires SearchTreeRec(sk)
+    ensures ValidRec(n, sk)
+    ensures SearchTreeRec(sk)
+    ensures b == exists n | n in elems(sk) :: n.key == k
+    ensures b ==> z in elems(sk) && z.key==k  
+
+    requires forall x | x in elems(sk) :: allocated(x)
+    ensures forall x {:trigger x in elems(sk), x in old(elems(sk))} | x in elems(sk) - old(elems(sk)) :: fresh(x)
+    ensures fresh(elems(sk)-old(elems(sk)))
+    ensures forall x | x in elems(sk) :: allocated(x)
+ 
+  method {:verify false} Search(k: K) returns (b:bool)
+    requires Valid()
+    requires SearchTree()
+    ensures Valid()
+    ensures SearchTree()
+    ensures b == (k in MapModel())
+
+    requires forall x | x in Repr() :: allocated(x)
+    ensures forall x | x in Repr() :: allocated(x)
+    ensures fresh(Repr()-old(Repr()))
+    ensures forall x | x in Repr() :: allocated(x)
+
+  static method {:verify false} GetRec(n: TNode, ghost sk: tree<TNode>, k: K) returns (v: V)
+    requires ValidRec(n, sk)
+    requires SearchTreeRec(sk)
+    //requires exists n | n in elems(sk) :: n.key == k
+    requires k in MapModelRec(sk)
+
+    ensures ValidRec(n, sk)
+    ensures SearchTreeRec(sk)
+    ensures exists n | n in elems(sk) :: n.key == k && n.value == v
+    ensures MapModelRec(sk)==old(MapModelRec(sk))
+    ensures MapModelRec(sk)[k]==v
+
+    requires forall x | x in elems(sk) :: allocated(x)
+    ensures forall x {:trigger x in elems(sk), x in old(elems(sk))} | x in elems(sk) - old(elems(sk)) :: fresh(x)
+    ensures fresh(elems(sk)-old(elems(sk)))
+    ensures forall x | x in elems(sk) :: allocated(x)
+  {
+    ModelRelationWithSkeletonKeyRec(n,sk,k);
+    assert exists n | n in elems(sk) :: n.key == k;
+    
+    if k == n.key {
+      v := n.value;
+    } else if n.key < k {
+      v := GetRec(n.right, sk.right, k);
+    } else if k < n.key {
+      v := GetRec(n.left, sk.left, k);
+    } else {
+      assert false;
+    }
+    ModelRelationWithSkeletonRecL(n,sk,k,v);
+    
+  }
+
+  method {:verify false} Get(k: K) returns (v: V)
+    requires Valid()
+    requires SearchTree()
+    requires k in MapModel()
+    ensures Valid()
+    ensures SearchTree()
+    ensures k in MapModel()
+    ensures MapModel()[k] == v
+
+    requires forall x | x in Repr() :: allocated(x)
+    ensures forall x | x in Repr() :: allocated(x)
+    ensures fresh(Repr()-old(Repr()))
+    ensures forall x | x in Repr() :: allocated(x)
+  {
+    assert Repr() == elems(skeleton);
+    v := GetRec(root, skeleton, k);
+  }
+
+  
+
+static lemma  pushUpMapL(ml:map<K,V>, mr:map<K,V>, k:K, v:V)  
+requires k !in mr
+ensures ml[k:=v]+mr == (ml+mr)[k:=v]
+{}
+
+static lemma  pushUpMapR(ml:map<K,V>, mr:map<K,V>, k:K, v:V)  
+ensures (ml+mr)[k:=v]==ml+mr[k:=v]
+{}
+
+static lemma  pushUpMapD(ml:map<K,V>, mr:map<K,V>, k:K)  
+requires k !in mr
+ensures ml-{k}+mr == (ml+mr)-{k}
+{}
+
+static lemma  pushUpMapDR(ml:map<K,V>, mr:map<K,V>, k:K)  
+requires k !in ml
+ensures ml+(mr-{k}) == (ml+mr)-{k}
+{}
+
+static lemma  deletion(m:map<K,V>, m':map<K,V>, k:K,v:V)  
+requires m==m'[k:=v] && k !in m'
+ensures m-{k}==m'
+{}
+
+static lemma idem(m:map<K,V>,k:K,v:V)
+requires k in m && m[k]==v
+ensures (m-{k})[k:=v]==m
+{}
+
+static lemma idem2(m:map<K,V>,k:K,v:V)
+requires k !in m 
+ensures (m[k:=v])-{k}==m
+{}
+
+static lemma keysSearchTree(sk:tree<TNode>,k:K)
+requires SearchTreeRec(sk)  && sk !=Empty()
+ensures (set n | n in elems(sk)::n.key) == MapModelRec(sk).Keys
+ensures sk.data.key !in MapModelRec(sk.left) && sk.data.key !in MapModelRec(sk.right)
+ensures MapModelRec(sk.left).Keys !! MapModelRec(sk.right).Keys 
+ensures MapModelRec(sk).Keys==MapModelRec(sk.left).Keys+MapModelRec(sk.right).Keys+{sk.data.key}
+ensures  k < sk.data.key ==> k !in MapModelRec(sk.right)
+ensures  k > sk.data.key ==> k !in MapModelRec(sk.left)
+{
+}
+
+static lemma keysSearchTreeP(sk:tree<TNode>)
+requires SearchTreeRec(sk)  && sk !=Empty()
+ensures (set n | n in elems(sk)::n.key) == MapModelRec(sk).Keys
+ensures sk.data.key !in MapModelRec(sk.left) && sk.data.key !in MapModelRec(sk.right)
+ensures MapModelRec(sk.left).Keys !! MapModelRec(sk.right).Keys 
+ensures MapModelRec(sk).Keys==MapModelRec(sk.left).Keys+MapModelRec(sk.right).Keys+{sk.data.key}
+{}
+
+static lemma {:verify false} oldNewMapModelRecL(newSk:tree<TNode>, moSk:map<K,V>,mskL:map<K,V>,mskR:map<K,V>,node:TNode,k:K,v:V)
+requires ValidRec(node,newSk) && SearchTreeRec(newSk)
+requires newSk!=Empty 
+requires MapModelRec(newSk.left)==mskL[k:=v]
+requires MapModelRec(newSk.right)==mskR
+requires node.key !in mskL && node.key !in mskR && node.key !=k && k !in mskR
+requires moSk==(mskL+mskR)[node.key:=node.value]
+ensures MapModelRec(newSk)==moSk[k:=v]
+{
+calc =={
+           MapModelRec(newSk);
+           (MapModelRec(newSk.left)+MapModelRec(newSk.right))[node.key:=node.value];
+           (mskL[k:=v]+mskR)[node.key:=node.value];
+           { pushUpMapR(mskL[k:=v],mskR,node.key,node.value);}
+           mskL[k:=v]+mskR[node.key:=node.value];
+           {  
+             assert k !in mskR[node.key:=node.value];
+             pushUpMapL(mskL,mskR[node.key:=node.value],k,v);}
+           ((mskL+mskR)[node.key:=node.value])[k:=v];
+           moSk[k:=v];
+
+}
+}
+
+
+static lemma {:verify false} oldNewMapModelRecR(newSk:tree<TNode>, moSk:map<K,V>,mskL:map<K,V>,mskR:map<K,V>,node:TNode,k:K,v:V)
+requires ValidRec(node,newSk) && SearchTreeRec(newSk)
+requires newSk!=Empty 
+requires MapModelRec(newSk.left)==mskL
+requires MapModelRec(newSk.right)==mskR[k:=v]
+requires node.key !in mskL && node.key !in mskR && node.key !=k
+requires moSk==(mskL+mskR)[node.key:=node.value]
+ensures MapModelRec(newSk)==moSk[k:=v]
+{
+calc =={
+           MapModelRec(newSk);
+           (MapModelRec(newSk.left)+MapModelRec(newSk.right))[node.key:=node.value];
+           (mskL+mskR[k:=v])[node.key:=node.value];
+           {pushUpMapR(mskL[k:=v],mskR,node.key,node.value);}
+           mskL+mskR[k:=v][node.key:=node.value];
+           {assert k != node.key;}
+           mskL+mskR[node.key:=node.value][k:=v];
+           {pushUpMapR(mskL,mskR[node.key:=node.value],k,v);}
+           ((mskL+mskR)[node.key:=node.value])[k:=v];
+           moSk[k:=v];
+
+}
+}
+
+
+
+ static method {:verify false} InsertRec(node: TNode?, ghost sk: tree<TNode>, k: K, v: V) returns (newNode: TNode, ghost newSk: tree<TNode>, ghost z:TNode)
+    modifies set x | x in elems(sk) :: x`left
+    modifies set x | x in elems(sk) :: x`right
+    modifies set x | x in elems(sk) :: x`value
+    requires ValidRec(node, sk)
+    requires SearchTreeRec(sk)
+    requires forall x | x in elems(sk) :: allocated(x)
+
+    ensures ValidRec(newNode, newSk)
+    ensures SearchTreeRec(newSk)
+    ensures MapModelRec(newSk)==old(MapModelRec(sk))[k:=v]
+
+    ensures elems(newSk)==elems(sk)+{z}
+    ensures z.key==k && z.value==v
+    ensures forall n | n in elems(sk) && old(n.key)!=k :: n.key==old(n.key) && n.value==old(n.value)
+    ensures forall x {:trigger x in elems(newSk), x in old(elems(newSk))} | x in elems(newSk) - old(elems(sk)) :: fresh(x)
+    ensures fresh(elems(newSk)-old(elems(sk)))
+    ensures forall x | x in elems(newSk) :: allocated(x)
+  {
+      
+    if node == null {
+      newNode := new TNode(null, k, v, null);
+      newSk := Node(Empty, newNode, Empty);
+      z:=newNode;
+    } else {
+       assert sk.data==node;
+
+      newNode := node;
+      if k == node.key {
+        node.value := v;
+        newSk := sk;
+        z:=node;
+      } else if node.key < k {
+
+        ghost var newSkRight;
+        node.right, newSkRight, z := InsertRec(node.right, sk.right, k, v);
+
+        newSk := Node(sk.left, node, newSkRight);
+
+      } else if k < node.key {
+
+        ghost var oMMRight:=MapModelRec(sk.right);
+        ghost var oMMLeft:=MapModelRec(sk.left);
+        ghost var oMM:=MapModelRec(sk);
+        keysSearchTree(sk,k);
+
+        ghost var newSkLeft;
+        node.left, newSkLeft,z := InsertRec(node.left, sk.left, k, v);
+
+
+        newSk := Node(newSkLeft, node, sk.right);
+        
+        assert node.key!=k;
+        assert node.key==old(node.key) && node.value==old(node.value);
+        assert node.key !in oMMLeft && node.key !in oMMRight && node.key !=k;
+
+        assert newSk.left==newSkLeft && newSk.right==sk.right && newSk.data==node;
+        assert MapModelRec(newSk.left)==oMMLeft[k:=v];
+        assert MapModelRec(newSk.right)==oMMRight;
+        assert oMM==(oMMLeft+oMMRight)[node.key:=node.value];
+        oldNewMapModelRecL(newSk,old(MapModelRec(sk)),oMMLeft,oMMRight,node,k,v);
+
+      } else {
+        assert false;
+      }
+    }
+  }
+  
+
+
+  method {:verify false} Insert(k: K, v: V)
+    modifies this, Repr()
+    requires Valid()
+    requires SearchTree()
+    ensures Valid()
+    ensures SearchTree()
+    ensures MapModel() == old(MapModel())[k := v]
+
+    requires forall x | x in Repr() :: allocated(x)
+    ensures forall x {:trigger x in Repr(), x in old(Repr())} | x in Repr() - old(Repr()) :: fresh(x)
+    ensures fresh(Repr()-old(Repr()))
+    ensures forall x | x in Repr() :: allocated(x)
+  {
+   
+    ghost var z;
+   
+    root, skeleton, z := InsertRec(root, skeleton, k, v);
+
+  }
+
+
+static lemma {:verify false} oldNewMapModelRecRemoveL(newSk:tree<TNode>, moSk:map<K,V>,mskL:map<K,V>,mskR:map<K,V>,node:TNode,k:K)
+requires ValidRec(node,newSk) && SearchTreeRec(newSk)
+requires newSk!=Empty 
+requires MapModelRec(newSk.left)==mskL-{k}
+requires MapModelRec(newSk.right)==mskR
+requires node.key !in mskL && node.key !in mskR && node.key !=k && k !in mskR
+requires moSk==(mskL+mskR)[node.key:=node.value]
+ensures MapModelRec(newSk)==moSk-{k}
+{
+  calc =={
+           MapModelRec(newSk);
+           (MapModelRec(newSk.left)+MapModelRec(newSk.right))[node.key:=node.value];
+           (mskL-{k}+mskR)[node.key:=node.value];
+           { assert node.key !in mskR;
+             pushUpMapR(mskL-{k},mskR,node.key,node.value);}
+           mskL-{k}+mskR[node.key:=node.value];
+           { assert k !in mskR[node.key:=node.value];
+             pushUpMapD(mskL,mskR[node.key:=node.value],k);}
+           ((mskL+mskR)[node.key:=node.value])-{k};
+           moSk-{k};
+  }
+}
+
+
+static lemma {:verify false} oldNewMapModelRecRemoveR(newSk:tree<TNode>, moSk:map<K,V>,mskL:map<K,V>,mskR:map<K,V>,node:TNode,k:K)
+requires ValidRec(node,newSk) && SearchTreeRec(newSk)
+requires newSk!=Empty 
+requires MapModelRec(newSk.left)==mskL
+requires MapModelRec(newSk.right)==mskR-{k}
+requires node.key !in mskL && node.key !in mskR && node.key !=k && k !in mskL
+requires moSk==(mskL+mskR)[node.key:=node.value]
+ensures MapModelRec(newSk)==moSk-{k}
+{
+  calc =={
+           MapModelRec(newSk);
+           (MapModelRec(newSk.left)+MapModelRec(newSk.right))[node.key:=node.value];
+           (mskL+(mskR-{k}))[node.key:=node.value];
+           { assert k !in mskL;
+             pushUpMapDR(mskL,mskR,k);}
+            ((mskL+mskR)-{k})[node.key:=node.value];
+           {assert node.key!=k;}
+           ((mskL+mskR)[node.key:=node.value])-{k};
+           moSk-{k};
+  }
+}
+
+static lemma {:verify false} oldNewMapModelRecRemoveRMin(newSk:tree<TNode>, moSk:map<K,V>,mskL:map<K,V>,mskR:map<K,V>,node:TNode,newNode:TNode)
+requires ValidRec(newNode,newSk) && SearchTreeRec(newSk)
+requires newSk!=Empty 
+requires MapModelRec(newSk.left)==mskL
+requires MapModelRec(newSk.right)==mskR-{newNode.key}
+requires node.key !in mskL && node.key !in mskR 
+requires newNode.key in mskR && mskR[newNode.key]==newNode.value
+requires moSk==(mskL+mskR)[node.key:=node.value] 
+ensures MapModelRec(newSk)==moSk-{node.key}
+{
+  calc =={
+           MapModelRec(newSk);
+           (MapModelRec(newSk.left)+MapModelRec(newSk.right))[newNode.key:=newNode.value];
+           (mskL+(mskR-{newNode.key}))[newNode.key:=newNode.value];
+           {pushUpMapR(mskL,mskR-{newNode.key},newNode.key,newNode.value);}
+           mskL+(mskR-{newNode.key})[newNode.key:=newNode.value];
+           {idem(mskR,newNode.key,newNode.value);}
+           mskL+mskR;
+           { 
+             idem2(mskL+mskR,node.key,node.value);}
+           ((mskL+mskR)[node.key:=node.value])-{node.key};
+           moSk-{node.key};
+  }
+}
+
+  static method {:verify false} RemoveMinRec(node: TNode, ghost sk: tree<TNode>) returns (newNode: TNode?, ghost newSk: tree<TNode>, removedNode: TNode)
+    modifies set x | x in elems(sk) :: x`left
+
+    requires ValidRec(node, sk)
+    requires SearchTreeRec(sk)
+    ensures ValidRec(newNode, newSk)
+    ensures SearchTreeRec(newSk)
+
+    ensures removedNode in elems(sk) && removedNode !in elems(newSk) 
+    ensures removedNode.key==old(removedNode.key) && removedNode.value==old(removedNode.value)
+    ensures elems(newSk) + {removedNode} == elems(sk)
+
+    ensures removedNode.key in old(MapModelRec(sk)) &&  old(MapModelRec(sk))[removedNode.key]==removedNode.value
+    ensures MapModelRec(newSk)==old(MapModelRec(sk))-{removedNode.key}
+
+    ensures forall n | n in elems(sk) :: n.key==old(n.key) && n.value==old(n.value)
+    ensures forall n | n in elems(sk) && n.key != removedNode.key :: removedNode.key < n.key
+    
+
+    requires forall x | x in elems(sk) :: allocated(x)
+    ensures forall x {:trigger x in elems(sk), x in old(elems(sk))} | x in elems(sk) - old(elems(sk)) :: fresh(x)
+    ensures fresh(elems(sk)-old(elems(sk)))
+    ensures forall x | x in elems(sk) :: allocated(x)
+  {      
+    keysSearchTreeP(sk);
+
+    if node.left == null {
+      ghost var oMMRight:=MapModelRec(sk.right);
+      ghost var oMM:=MapModelRec(sk);
+      
+      deletion(oMM,oMMRight,node.key,node.value);
+
+      newNode := node.right;
+      newSk := sk.right;
+      removedNode := node;
+      
+    } else {
+      ghost var oMMRight:=MapModelRec(sk.right);
+      ghost var oMMLeft:=MapModelRec(sk.left);
+      ghost var oMM:=MapModelRec(sk);
+
+      ghost var newSkLeft;
+      node.left, newSkLeft, removedNode := RemoveMinRec(node.left, sk.left);
+      
+      newNode:=node;      
+      newSk := Node(newSkLeft, newNode, sk.right);
+
+      oldNewMapModelRecRemoveL(newSk,oMM,oMMLeft,oMMRight,node,removedNode.key);
+    }
+  }
+
+  static method {:verify false} RemoveRec(node: TNode?, ghost sk: tree<TNode>, k: K) returns (newNode: TNode?, ghost newSk: tree<TNode>, ghost removedNode: TNode?)
+    modifies set x | x in elems(sk) :: x`left
+    modifies set x | x in elems(sk) :: x`right
+    requires ValidRec(node, sk)
+    requires SearchTreeRec(sk)
+    ensures ValidRec(newNode, newSk)
+    ensures SearchTreeRec(newSk)
+   
+    ensures forall n | n in elems(sk) :: n.key == old(n.key) && n.value == old(n.value)
+    ensures elems(newSk) == elems(sk) - {removedNode}
+    ensures k !in old(MapModelRec(sk)) <==> removedNode==null 
+    ensures removedNode != null ==> removedNode in elems(sk) && removedNode !in elems(newSk) && removedNode.key == k
+    ensures MapModelRec(newSk)==old(MapModelRec(sk))-{k}
+  
+    requires forall x | x in elems(sk) :: allocated(x)
+    ensures forall x {:trigger x in elems(sk), x in old(elems(sk))} | x in elems(sk) - old(elems(sk)) :: fresh(x)
+    ensures fresh(elems(sk)-old(elems(sk)))
+    ensures forall x | x in elems(sk) :: allocated(x)
+  {
+       ModelRelationWithSkeletonKeyRec(node,sk,k);
+
+    if node == null {
+      newNode := node;
+      newSk := sk;
+      removedNode := null;
+      assert MapModelRec(newSk)==old(MapModelRec(sk))-{k};
+    } else {
+       ghost var oMMRight:=MapModelRec(sk.right);
+       ghost var oMMLeft:=MapModelRec(sk.left);
+       ghost var oMM:=MapModelRec(sk);
+       keysSearchTreeP(sk);
+       assert node.key !in oMMLeft && node.key !in oMMRight;
+
+      if node.key < k {
+        ghost var newSkRight;
+        node.right, newSkRight, removedNode := RemoveRec(node.right, sk.right, k);
+        newNode := node;
+        newSk := Node(sk.left, node, newSkRight);
+        
+        assert MapModelRec(newSkRight)==oMMRight-{k};
+        oldNewMapModelRecRemoveR(newSk,oMM,oMMLeft,oMMRight,node,k);
+        assert MapModelRec(newSk)==old(MapModelRec(sk))-{k};
+
+      } else if k < node.key {
+        newNode := node;
+        ghost var newSkLeft;
+        node.left, newSkLeft, removedNode := RemoveRec(node.left, sk.left, k);
+        newSk := Node(newSkLeft, node, sk.right);
+        
+        assert MapModelRec(newSkLeft)==oMMLeft-{k};
+        oldNewMapModelRecRemoveL(newSk,oMM,oMMLeft,oMMRight,node,k);
+        assert MapModelRec(newSk)==old(MapModelRec(sk))-{k};
+
+      } else {
+        assert k == node.key;
+        if node.right == null {
+          newNode := node.left;
+          newSk := sk.left;
+          removedNode := node;
+          
+          assert oMM==oMMLeft[node.key:=node.value] && node.key !in oMMLeft;
+          deletion(oMM,oMMLeft,node.key,node.value);
+          assert MapModelRec(newSk)==old(MapModelRec(sk))-{k};
+
+        } else if node.left == null {
+          newNode := node.right;
+          newSk := sk.right;
+          removedNode := node;
+          
+          assert oMM==oMMRight[node.key:=node.value] && node.key !in oMMRight;
+          deletion(oMM,oMMRight,node.key,node.value);
+          assert MapModelRec(newSk)==old(MapModelRec(sk))-{k};
+
+        } else {
+          removedNode := node;
+          ghost var newSkRight;
+          var newRight;
+          newRight, newSkRight, newNode := RemoveMinRec(node.right, sk.right);
+          
+          assert MapModelRec(newSkRight)==oMMRight-{newNode.key};
+          assert newNode.key in oMMRight && oMMRight[newNode.key]==newNode.value;
+
+          
+          newNode.left := node.left;
+          newNode.right := newRight;
+          newSk := Node(sk.left, newNode, newSkRight);
+
+
+          oldNewMapModelRecRemoveRMin(newSk,oMM,oMMLeft,oMMRight,node,newNode);
+          assert MapModelRec(newSk)==old(MapModelRec(sk))-{k};
+
+        }
+      }
+    }
+  }
+
+  method {:verify false} Remove(k: K)
+    modifies this, Repr()
+    requires Valid()
+    requires SearchTree()
+    ensures Valid()
+    ensures SearchTree()
+    ensures MapModel()==old(MapModel())-{k}
+
+    requires forall x | x in Repr() :: allocated(x)
+    ensures forall x {:trigger x in Repr(), x in old(Repr())} | x in Repr() - old(Repr()) :: fresh(x)
+    ensures fresh(Repr()-old(Repr()))
+    ensures forall x | x in Repr() :: allocated(x)
+  {
+    ghost var removedNode;
+    root, skeleton, removedNode := RemoveRec(root, skeleton, k);
+  }
+
+  
+}
