src/tree/layer3/OrderedMultisetImpl.dfy
@@ -1,0 +1,418 @@
+include "../../../src/tree/layer1/OrderedMultiset.dfy"
+include "../../../src/tree/layer1/OrderedMultisetUtils.dfy"
+include "../../../src/tree/BinTreeIntClara.dfy"
+
+
+class OrderedMultisetIteratorImplMap extends OrderedMultisetIterator{
+  
+  // ghost var parent:UnorderedMultiset;
+   
+  function Parent(): UnorderedMultiset
+    reads this
+  //{ parent } 
+
+  predicate Valid()
+    reads this, Parent(), Parent().Repr()
+  //{ true }
+
+  function Traversed():multiset<int>
+    reads this, Parent(), Parent().Repr()
+    requires Valid()
+    requires Parent().Valid() 
+    ensures Traversed()<=Parent().Model()
+    ensures forall x,y | x in Traversed() && y in Parent().Model()-Traversed() :: x<=y
+
+   //Several elements equal to the Peek may be in Traversed and some others not
+  // Example: Model=={1,1,2,3,3,3,4,5} Traversed=={1,1,2,3,3} Peek=3 
+
+  function method Peek(): int
+    reads this, Parent(), Parent().Repr()
+    requires Valid()
+    requires Parent().Valid()
+    requires HasNext()
+    ensures Peek() in Parent().Model() && (Parent().Model()-Traversed())[Peek()]>0
+    ensures Peek()==elemth(Parent().Model(),|Traversed()|)
+    ensures forall x | x in Traversed() :: x<=Peek()
+    ensures forall x | x in Parent().Model()-Traversed() :: Peek()<=x 
+
+
+  function method Index(): int
+    reads this, Parent(), Parent().Repr()
+    requires Valid()
+    requires Parent().Valid()
+    ensures HasNext() ==> Index()==|Traversed()|
+    ensures !HasNext() ==> Index()==|Parent().Model()|
+   
+  function method HasNext(): bool
+    reads this, Parent(), Parent().Repr()
+    requires Valid()
+    requires Parent().Valid()
+    ensures HasNext()  <==> Traversed() < Parent().Model() && |Traversed()| < |Parent().Model()|
+    //|Traversed()| < |Parent().Model()| es necesario para poder verificar con cota |s.Model()|-|it.Traversed()|
+    ensures !HasNext() ==> Traversed() == Parent().Model() && |Traversed()| == |Parent().Model()|
+  //{ true }
+
+  method Next() returns (x: int)
+    modifies this
+    requires Valid()
+    requires Parent().Valid()
+    requires HasNext()
+    requires allocated(Parent())
+    requires forall it | it in Parent().Repr() :: allocated(it)
+    ensures Parent().Valid()
+    ensures Valid()
+    ensures old(Parent()) == Parent()
+    ensures old(Parent().Model()) == Parent().Model()
+
+    ensures forall x {:trigger x in Parent().Repr(), x in old(Parent().Repr())} | x in Parent().Repr() - old(Parent().Repr()) :: fresh(x)
+    ensures fresh(Parent().Repr()-old(Parent().Repr()))
+    ensures forall x | x in Parent().Repr() :: allocated(x)
+
+    ensures Parent().Iterators() == old(Parent().Iterators())
+    ensures x==old(Peek()) && Traversed() == multiset{old(Peek())}+old(Traversed()) 
+    ensures |Traversed()|==1+|old(Traversed())|
+    ensures HasNext() ==> Peek()==elemth(Parent().Model(),|Traversed()|)//already known
+
+
+    ensures forall it | it in Parent().Iterators() && old(it.Valid()) ::
+      it.Valid() && (it != this ==> it.Traversed() == old(it.Traversed()) && (it.HasNext() ==> it.Peek()==old(it.Peek())))
+
+  function method HasPrev(): bool//igual que HasNext
+    reads this, Parent(), Parent().Repr()
+    requires Valid()
+    requires Parent().Valid()
+    ensures HasPrev()  <==> Traversed() < Parent().Model() && |Traversed()| < |Parent().Model()|
+    //|Traversed()| < |Parent().Model()| es necesario para poder verificar con cota |s.Model()|-|it.Traversed()|
+    ensures !HasPrev() ==> Traversed() == Parent().Model() && |Traversed()| == |Parent().Model()|
+  
+
+  method Prev() returns (x: int)
+    modifies this
+    requires Valid()
+    requires Parent().Valid()
+    requires HasNext() 
+    requires allocated(Parent())
+    requires forall it | it in Parent().Repr() :: allocated(it)
+    ensures Parent().Valid()
+    ensures Valid()
+    ensures old(Parent()) == Parent()
+    ensures old(Parent().Model()) == Parent().Model()
+
+    ensures forall x {:trigger x in Parent().Repr(), x in old(Parent().Repr())} | x in Parent().Repr() - old(Parent().Repr()) :: fresh(x)
+    ensures fresh(Parent().Repr()-old(Parent().Repr()))
+    ensures forall x | x in Parent().Repr() :: allocated(x)
+
+    ensures Parent().Iterators() == old(Parent().Iterators())
+    ensures x==old(Peek())  
+    ensures old(Traversed())==multiset{} ==> Traversed()==Parent().Model()
+    ensures old(Traversed())!=multiset{} ==> Traversed()==old(Traversed())-multiset{maximum(old(Traversed()))}
+    ensures forall it | it in Parent().Iterators() && old(it.Valid()) ::
+      it.Valid() && (it != this ==> it.Traversed() == old(it.Traversed()) && (it.HasNext() ==> it.Peek()==old(it.Peek())))
+
+  method Copy() returns (it: UnorderedMultisetIterator)
+    modifies Parent(), Parent().Repr()
+    requires Valid()
+    requires Parent().Valid()
+    requires allocated(Parent())
+    requires forall it | it in Parent().Iterators() :: allocated(it)
+    ensures fresh(it)
+    ensures Valid()
+    ensures Parent() == old(Parent())
+    ensures Parent().Valid()
+    ensures Parent().Model() == old(Parent().Model())
+
+    ensures forall x {:trigger x in Parent().Repr(), x in old(Parent().Repr())} | x in Parent().Repr() - old(Parent().Repr()) :: fresh(x)
+    ensures fresh(Parent().Repr()-old(Parent().Repr()))
+    ensures forall x | x in Parent().Repr() :: allocated(x)
+    
+    ensures it is OrderedMultisetIterator
+    ensures it.Valid()
+    ensures Parent().Iterators() == {it} + old(Parent().Iterators())
+    ensures Parent() == it.Parent()
+
+    ensures Traversed() == it.Traversed() 
+    ensures HasNext() ==> Peek()==it.Peek()
+    ensures forall it | it in old(Parent().Iterators()) && old(it.Valid()) ::
+      it.Valid() && it.Traversed() == old(it.Traversed()) && (it.HasNext() ==> it.Peek()==old(it.Peek()))
+
+  
+}
+
+class OrderedMultisetImplMap extends OrderedMultiset{
+  
+  var  tree:Tree;
+  ghost var iters:set<OrderedMultisetIteratorImplMap>;
+
+
+  constructor()
+  {
+   tree:=new Tree();
+   iters:={};
+
+  }
+
+  function Repr0(): set<object>
+    reads this
+  {
+    {tree} + iters 
+  }
+
+  function ReprDepth(): nat
+    ensures ReprDepth() > 0
+  { 1 }
+
+  function ReprFamily(n: nat): set<object>
+    decreases n
+    requires n <= ReprDepth()
+    ensures n > 0 ==> ReprFamily(n) >= ReprFamily(n-1)
+    reads this, if n == 0 then {} else ReprFamily(n-1)
+  {
+    if (n==0) then Repr0()
+    else Repr0()+tree.Repr()
+  }
+  
+
+  lemma UselessLemma()
+    ensures Repr() == ReprFamily(ReprDepth());
+
+  predicate Valid()
+    reads this, Repr()
+  {
+   tree.Valid() && tree.SearchTree() 
+   && forall p | p in tree.MapModel().Items:: p.1>0
+  }  
+
+
+
+  function mapToMultiset(s:set<(K,V)>):multiset<K>
+  //requires forall p1,p2 | p1 in s && p2 in s && p1!=p2 :: p1.0!=p2.0
+  requires forall p | p in s :: p.1>0
+  {
+    if (s=={}) then multiset{}
+    else 
+       var p:| p in s;
+       //assert p.1>0 && p.0 !in mapToMultiset(s-{p});
+       mapToMultiset(s-{p})[p.0:=p.1]
+
+  }
+  function Model(): multiset<int>
+    reads this, Repr()
+    requires Valid()
+  {
+    mapToMultiset(tree.MapModel().Items)
+  }
+
+  function method Empty(): bool
+    reads this, Repr()
+    requires Valid()
+    ensures Empty() <==> Model() == multiset{}
+  {
+   tree.isEmpty()
+  }
+
+  function method Size(): nat
+    reads this, Repr()
+    requires Valid()
+    ensures Size() == |Model()|
+  //La suma de las multiplicidades
+
+  function Iterators(): set<UnorderedMultisetIterator>
+    reads this, Repr()
+    requires Valid()
+    ensures forall it | it in Iterators() :: it in Repr() && it.Parent() == this
+    ensures forall it | it in Iterators() :: it is OrderedMultisetIterator
+    { {} }
+
+  method First() returns (it: UnorderedMultisetIterator)
+    modifies this, Repr()
+    requires Valid()
+    requires forall x | x in Repr() :: allocated(x)
+    ensures Valid()
+    ensures Model() == old(Model())
+
+    ensures forall x {:trigger x in Repr(), x in old(Repr())} | x in Repr() - old(Repr()) :: fresh(x)
+    ensures fresh(Repr()-old(Repr()))
+    ensures forall x | x in Repr() :: allocated(x)
+
+    ensures it is OrderedMultisetIterator
+    ensures fresh(it)
+    ensures Iterators() == {it} + old(Iterators())
+    ensures it.Valid()
+    ensures it.Parent() == this
+    ensures it.Traversed()==multiset{} 
+    ensures Model()!=multiset{} ==> it.HasNext() && it.Peek()==elemth(Model(),0)
+    ensures forall it | it in old(Iterators()) && old(it.Valid()) ::
+      it.Valid() && it.Traversed() == old(it.Traversed()) && (it.HasNext() ==> it.Peek()==old(it.Peek()))
+
+
+  method Last() returns (it: OrderedMultisetIterator)//iterator to the last element
+    modifies this, Repr()
+    requires Valid()
+    requires forall x | x in Repr() :: allocated(x)
+    ensures Valid()
+    ensures Model() == old(Model())
+
+    ensures forall x {:trigger x in Repr(), x in old(Repr())} | x in Repr() - old(Repr()) :: fresh(x)
+    ensures fresh(Repr()-old(Repr()))
+    ensures forall x | x in Repr() :: allocated(x)
+
+    ensures fresh(it)
+    ensures Iterators() == {it} + old(Iterators())
+    ensures it.Valid()
+    ensures it.Parent() == this
+    ensures Model()!=multiset{} ==> it.HasNext() && it.Traversed()==Model()-multiset{elemth(Model(),|Model()|-1)} && it.Peek()==elemth(Model(),|Model()|-1)
+    ensures Model()==multiset{} ==> it.Traversed()==multiset{}
+    ensures forall it | it in old(Iterators()) && old(it.Valid()) ::
+      it.Valid() && it.Traversed() == old(it.Traversed()) && (it.HasNext() ==> it.Peek()==old(it.Peek()))
+  
+  function contains(x:int):bool
+    reads this, Repr()
+    requires Valid()
+    ensures  contains(x) == (x in Model())
+
+  method count(x:int) returns (c:int)
+    requires Valid()
+    ensures Valid() && c==Model()[x]  
+  {
+   var b:=tree.Search(x);
+   if (b) 
+     {
+       c:=tree.Get(x);
+     }
+   else 
+     { c:=0; }
+
+  }
+  
+  method add(x:int)
+    modifies this,Repr()
+    requires Valid()
+    requires forall x | x in Repr() :: allocated(x)
+    ensures Valid()
+    ensures Model() == old(Model()) + multiset{x} 
+
+    ensures forall x {:trigger x in Repr(), x in old(Repr())} | x in Repr() - old(Repr()) :: fresh(x)
+    ensures fresh(Repr()-old(Repr()))
+    ensures forall x | x in Repr() :: allocated(x)
+   
+    ensures Iterators() == old(Iterators())
+  /*{
+   if (!contains(x)) {tree.Insert(x,1);}
+   else {
+     var c:=tree.Get(x);
+     tree.Insert(x,c+1);
+   }
+  }*/
+
+
+  method find(x:int) returns (newt:UnorderedMultisetIterator )
+    modifies this, Repr()
+    requires Valid()
+    requires forall x | x in Repr() :: allocated(x)
+    ensures Valid() 
+    ensures Model()==old(Model())
+
+    ensures newt is OrderedMultisetIterator
+    ensures fresh(newt) 
+    ensures newt.Valid() && newt.Parent()==this
+    ensures x in Model() ==> newt.HasNext() && newt.Traversed()==msmaller(Model(),x) && newt.Peek()==x //points to the first occurrence
+    ensures x !in Model() ==> newt.Traversed()==Model()
+
+    ensures forall x {:trigger x in Repr(), x in old(Repr())} | x in Repr() - old(Repr()) :: fresh(x)
+    ensures fresh(Repr()-old(Repr()))
+    ensures forall x | x in Repr() :: allocated(x)
+
+    ensures Iterators() == {newt}+old(Iterators())
+
+  method insert(mid: UnorderedMultisetIterator, x: int) returns (newt:UnorderedMultisetIterator)
+    modifies this, Repr()
+    requires Valid()
+    requires mid.Valid() 
+    //mid just a hint, it is inserted where corresponds
+    //efficiently or not if it respects order
+    requires mid.Parent() == this
+    requires mid in Iterators()
+    requires forall x | x in Repr() :: allocated(x)
+    ensures Valid()
+    ensures Model() == old(Model()) + multiset{x}
+
+    
+    ensures newt is OrderedMultisetIterator
+    ensures fresh(newt)
+    ensures Iterators() == {newt}+old(Iterators())
+    ensures newt.Valid() && newt.Parent()==this
+    ensures newt.HasNext() && 
+            msmaller(Model(),x)<=newt.Traversed()<=msmaller(Model(),x)[x:=old(Model())[x]] &&
+            newt.Peek()==x 
+            //Example: 1,2,2,2,2,3 insert another 2 , Traversed may be 
+            //{1} (newt points to the first 2), {1,2}, ..., {1,2,2,2,2} (newt points to the last 2)
+    
+    ensures forall x {:trigger x in Repr(), x in old(Repr())} | x in Repr() - old(Repr()) :: fresh(x)
+    ensures fresh(Repr()-old(Repr()))
+    ensures forall x | x in Repr() :: allocated(x)
+
+    //points either to the inserted elemento or to the already existing one
+
+
+
+  method remove(x:int) 
+    modifies this,Repr()
+    requires Valid()
+    requires forall x | x in Repr() :: allocated(x)
+    ensures Valid()
+    ensures Model()== old(Model()) - multiset{x} 
+
+    ensures forall x {:trigger x in Repr(), x in old(Repr())} | x in Repr() - old(Repr()) :: fresh(x)
+    ensures fresh(Repr()-old(Repr()))
+    ensures forall x | x in Repr() :: allocated(x)
+
+    ensures Iterators() == old(Iterators())
+  /*{
+    if (contains(x))
+    {
+     var c:=tree.Get(x);
+     if (c-1 != 0) { tree.Insert(x,c-1);}
+    }
+   
+  }*/
+
+  method removeAll(x:int) 
+    modifies this,Repr()
+    requires Valid()
+    requires forall x | x in Repr() :: allocated(x)
+    ensures Valid()
+    ensures Model()== old(Model())[x:=0] 
+
+    ensures forall x {:trigger x in Repr(), x in old(Repr())} | x in Repr() - old(Repr()) :: fresh(x)
+    ensures fresh(Repr()-old(Repr()))
+    ensures forall x | x in Repr() :: allocated(x)
+
+    ensures Iterators() == old(Iterators())
+   /*{
+     tree.Remove(x);
+   }*/
+  method erase(mid:UnorderedMultisetIterator) returns (next: UnorderedMultisetIterator)
+    modifies this, Repr()
+    requires Valid()
+    requires mid.Valid()
+    requires mid.Parent() == this
+    requires mid.HasNext()
+    requires mid in Iterators()
+    requires forall x | x in Repr() :: allocated(x)
+    ensures Valid()
+    ensures Model()== old(Model())-multiset{old(mid.Peek())}
+    
+    ensures next is OrderedMultisetIterator
+    ensures fresh(next)
+    ensures Iterators() == {next}+old(Iterators())
+    ensures next.Valid() && next.Parent()==this 
+    ensures next.Traversed()==old(mid.Traversed())  &&
+           (next.HasNext() ==> next.Peek()==elemth(Model(),|next.Traversed()|))
+
+    ensures forall x {:trigger x in Repr(), x in old(Repr())} | x in Repr() - old(Repr()) :: fresh(x)
+    ensures fresh(Repr()-old(Repr()))
+    ensures forall x | x in Repr() :: allocated(x)
+
+}
+
+
